Arithmetic/theories/Languages/MiniGMP/Lemmas.v
@@ -16,84 +16,104 @@ Section GMPLemmas.
 
     
 
-    Lemma _LC21_weakening_of_gmp_statement_semantics :
+    Lemma _LC21_weakening_of_gmp_statement_semantics_strong :
         _LC21_weakening_of_statement_semantics Empty_exp_sem _gmp_stmt_sem
-            exist_strong_env_mem_partial_order strong_env_mem_partial_order (fe:=fe)
+            exist_strong_env_mem_partial_order strong_env_mem_partial_order (fe:=fe) (ext_ty_val := _type_of_gmp)
     .
     Proof with eauto using refl_env_mem_partial_order with rac_hint ; try easy.
-        intros _ ev₀ s ev₁ Hderiv. 
+        intros _ _ ev₀ s ev₁ Hderiv. 
+        epose proof (fun y => weakening_of_c_expression_semantics y ev₀) as weak_exp.
         induction Hderiv; intros ev₀' sub Hstrenvmem; apply strong_env_mem_stronger in Hstrenvmem as Henvmem; 
-            epose proof (fun y => weakening_of_c_expression_semantics y ev₀) as weak_exp;
-            pose proof (eq_defined_mpz_mem_partial_order ev₀ ev₀' sub Henvmem) as eq_defined ;
-            pose proof (eq_mpz_env_mem_partial_order ev₀ ev₀' sub Henvmem) as  eq_mpz ;
-            pose proof (mem_def_partial_order_add) as mpz_add;
-            pose proof (env_partial_order_add ev₀ ev₀' sub Henvmem) as env_add.
+            pose proof (eq_defined_mpz_mem_partial_order _ _ _ Henvmem) as eq_defined ;
+            pose proof (eq_mpz_env_partial_order _ _ _ (proj1 Henvmem)) as eq_mpz ;
+            pose proof (env_partial_order_add_strong _ _ _ (proj1 Hstrenvmem)) as env_add.
 
         (* init *)
-        - clear weak_exp eq_defined eq_mpz env_add. 
-            exists (ev₀'    <| env ; vars ::= {{x \ Def (VMpz (Some (proj1_sig sub l)))}} |> 
-                            <| mstate ::= {{proj1_sig sub l \Defined 0}} |> ).
+        - clear weak_exp eq_defined eq_mpz. 
+            exists (ev₀'    <| env ; vars ::= {{x \ Def (VMpz (Some (sub l)))}} |> 
+                            <| mstate ::= {{sub l \Defined 0}} |> ).
             split.
-            + admit. (* now apply mpz_add. *)
-            + clear mpz_add. apply S_init with u.
-                * intros v. admit.
-                * destruct Hstrenvmem as [e m]. now apply e in H0.
+            * split ; simpl. 
+                -- apply env_add.
+                -- apply mem_partial_order_add. apply Henvmem.
+
+            * clear env_add . apply S_init with u. 
+                -- intros v Hcontra.
+                (* if ev0' v is bound to (sub l), the strong relation implies ev0 was bound to l, so it can't be a fresh location *)
+                enough (Hldef : ev₀ v = Some (Def (VMpz (Some l)))); [congruence|]. 
+                destruct Hstrenvmem as [Hstrenv _]. 
+                specialize (Hstrenv x v (VMpz l)). simpl in Hstrenv.
+                admit.
+                -- destruct Hstrenvmem as [e m]. now apply e in H0.
                     
         (* clear *)
         - exists (ev₀'  <| env ; vars ::= {{x\Def (VMpz None)}} |>
-                        <| mstate ::= {{(proj1_sig sub) a \ Undefined u}} |>). split.
-            + admit. (* now apply mpz_add. *)
+                        <| mstate ::= {{sub a \ Undefined u}} |>). split.
+            + split; simpl.
+                * apply env_add.
+                * apply mem_partial_order_add. apply Henvmem.
             + apply S_clear. now apply (eq_mpz x (Some a)).
 
         (* set_i *)
-        - exists (ev₀' <| mstate ::= {{(proj1_sig sub) a \ Defined (z) ̇}} |>).  split...
-            +  admit.
+        - exists (ev₀' <| mstate ::= {{sub a \ Defined (z) ̇}} |>).  split.
+            + split; simpl.
+                * apply Hstrenvmem.
+                * apply mem_partial_order_add. apply Henvmem.
             + apply S_set_i...
                 * now apply (eq_mpz x (Some a)).
                 * apply weak_exp... now exists sub.
 
         (* set_z *)
-        - exists (ev₀' <| mstate ::= {{(proj1_sig sub) a \Defined z}} |>). split...
-            + admit.
-            + apply S_set_z with (proj1_sig sub n)...
+        - exists (ev₀' <| mstate ::= {{sub a \Defined z}} |>). split.
+            + split; simpl.
+                * apply Hstrenvmem.
+                * apply mem_partial_order_add. apply Henvmem.
+            + apply S_set_z with (sub n)...
                 * now apply (eq_mpz x (Some a)).
                 * now apply (eq_mpz y (Some n)).
 
         (* get_int *)
-        -  exists (ev₀' <| env ; vars ::= fun e =>  e{x \ Def (VInt (zy ⁱⁿᵗ ir))} |>). split... 
-            + admit.
-            + apply S_get_int with (proj1_sig sub ly)... now apply (eq_mpz y (Some ly)).
+        -  exists (ev₀' <| env ; vars ::= fun e =>  e{x \ Def (VInt (zy ⁱⁿᵗ ir))} |>). split. 
+            + split; simpl.
+                * apply env_add. 
+                * apply Henvmem.
+            + apply S_get_int with (sub ly)... now apply (eq_mpz y (Some ly)).
         
         (* set_s *)
-        - exists (ev₀' <| mstate ::= {{(proj1_sig sub) lx \ Defined zx}} |>). split... 
-            + admit.
-            + constructor... now apply (eq_mpz x (Some lx)).
+        - exists (ev₀' <| mstate ::= {{sub lx \ Defined zx}} |>). split. 
+            + split; simpl.
+                * apply Hstrenvmem. 
+                * apply mem_partial_order_add. apply Henvmem.
+            +  constructor... now apply (eq_mpz x (Some lx)).
 
         (* cmp *)
-        -  exists (ev₀' <| env ; vars ::= fun e => e{c \induced (proj1_sig sub) b} |>).  split ... 
-            + admit.
-            + apply S_cmp with (proj1_sig sub lx) (proj1_sig sub ly) zx zy...
+        -  exists (ev₀' <| env ; vars ::= fun e => e{c \induced sub b} |>).  split.
+            + split; simpl.
+                * apply env_add. 
+                * apply Henvmem.
+            + apply S_cmp with (sub lx) (sub ly) zx zy...
                 * now apply (eq_mpz x (Some lx)).
                 * now apply (eq_mpz y (Some ly)).
                 * now apply cmp_induced.
         (* op *)
-        - eexists (ev₀' <| mstate ::= {{(proj1_sig sub) lr \Defined (⋄ bop zx zy)}} |>). split. 
-            + admit. (* now apply (mem_def_partial_order_add). *)
-            + apply S_op with (proj1_sig sub lx) (proj1_sig sub ly)...
+        - eexists (ev₀' <| mstate ::= {{sub lr \Defined (⋄ bop zx zy)}} |>). split. 
+            + split; simpl.
+                * apply Hstrenvmem. 
+                * apply mem_partial_order_add. apply Henvmem.
+            + apply S_op with (sub lx) (sub ly)...
                 * now apply (eq_mpz x (Some lx)).
                 * now apply (eq_mpz y (Some ly)).
-                * now apply (eq_mpz r (Some lr)).
+                * now apply (eq_mpz r (Some lr)). 
     Admitted.
 
 
 
-    Definition LC21_weakening_of_gmp_statement_semantics := 
+    Definition LC21_weakening_of_gmp_statement_semantics_strong := 
         LC21_weakening_of_statement_semantics_strong Empty_exp_sem _gmp_stmt_sem 
-        _determinist_gmp_stmt_eval
         weakening_of_empty_expression_semantics
-        _LC21_weakening_of_gmp_statement_semantics
+        _LC21_weakening_of_gmp_statement_semantics_strong
         (LC1_weakening_of_expression_semantics Empty_exp_sem weakening_of_empty_expression_semantics)
-        (ext_used_stmt_vars:=_gmp_used_stmt_vars) (ext_ty_val:=_type_of_gmp) (fe:=fe)
+        (ext_used_stmt_vars:=_gmp_used_stmt_vars) (ext_ty_val:=_type_of_gmp) (fe:=fe)        
     .
     
 
@@ -118,12 +138,14 @@ Section GMPLemmas.
             ev x = Some (Def (VMpz v'')) ->
             ev' x = Some (Def (VMpz (Some v'))) ->
             fresh_location ev  v  ->
-            ev'.(mstate) (proj1_sig sub v) = (ev' <| env;vars ::=e |> <| mstate ::= {{v'\val}} |>).(mstate) (proj1_sig sub v)
+            ev'.(mstate) (sub v) = (ev' <| env;vars ::=e |> <| mstate ::= {{v'\val}} |>).(mstate) (sub v)
             ). {
-            intros ev ev' v v' v'' val x e Henvmem Hnotused Hev Hev'. destruct (eq_dec (proj1_sig sub v) v').
+            intros ev ev' v v' v'' val x e Henvmem Hnotused Hev Hev'. destruct (eq_dec (sub v) v').
             - subst. exfalso. destruct Henvmem as [Henv _]. specialize (Henv x). 
                 inversion Henv;  try congruence.  rewrite Hev in H0. inversion H0. destruct sub. simpl in *.
-                apply bijective_eq_iff_f_eq in H2... subst. eapply Hev'...
+                apply bijective_eq_iff_f_eq in H2.
+                + subst. eapply Hev'...
+                + apply bij_wit_is_bij...
             - symmetry. now apply p_map_not_same_eq.
         }
 
@@ -134,7 +156,7 @@ Section GMPLemmas.
         (* init *)
         - split.
             + intros. eapply Hvars... 
-            + intros l' Hnotused. destruct (eq_dec (proj1_sig sub l') l0).
+            + intros l' Hnotused. destruct (eq_dec (sub l') l0).
                 * subst. exfalso.  admit. 
                     (* not provable, requires stronger Hnotused hypothesis *)
                 * symmetry. now apply p_map_not_same_eq.
@@ -186,21 +208,21 @@ Section GMPLemmas.
             (ext_used_stmt_vars := _gmp_used_stmt_vars) (fe:=fe) 
     .
     Proof with eauto using refl_env_mem_partial_order with rac_hint ; try easy.
-        intros ev s ev1 [sub [subrev [Hsub1 Hsub2]]] Hderiv. 
-        induction Hderiv; intros ev' Hrel [Henv Hmem].
+        intros ev s ev1 [sub subrev] Hderiv. 
+        induction Hderiv; intros ev' Hrel Henv Hmem.
         (* todo: factorize *)
 
         (* init *)
         - exists (ev' <| env ; vars ::= {{x \ Def (VMpz (Some (subrev l)))}} |> <| mstate ::= {{subrev l \Defined 0}} |> ).
             apply S_init with u.
             + intros x'. specialize (H x'). intros contra. destruct Hrel as [Hrel _]. specialize (Hrel x _ _ contra). simpl in *.  
-                inversion Hrel. congruence.
+                inversion Hrel. destruct Hbij; congruence.
 
             +  assert (~(dom ev - dom ev')%dom_ x). {
                 intros contra. apply Henv in contra. apply contra. simpl. StringSet.D.fsetdec. 
                 }
                 apply not_in_sub_domain_prop in H1;[|apply in_domain_dec| apply in_domain_dec]. destruct H1.
-                * now unshelve epose proof (strong_reverse_dom_same_env ev' ev x (UMpz u) sub subrev Hsub1 Hsub2 Hrel _ H1).
+                * now unshelve epose proof (strong_reverse_dom_same_env ev' ev x (UMpz u) sub subrev Hbij Hrel _ H1).
                 * exfalso. apply H1. now exists (UMpz u).
         
         (* clear *)
@@ -209,7 +231,7 @@ Section GMPLemmas.
                 intros contra. apply Henv in contra. apply contra. simpl. StringSet.D.fsetdec.
             }
             apply not_in_sub_domain_prop in H0;[|apply in_domain_dec| apply in_domain_dec]. destruct H0.
-            * now unshelve epose proof (strong_reverse_dom_same_env ev' ev x a sub subrev Hsub1 Hsub2 Hrel _ H0).
+            * now unshelve epose proof (strong_reverse_dom_same_env ev' ev x a sub subrev Hbij Hrel _ H0).
             * exfalso. apply H0. now exists a.
 
         (* set_i *)
@@ -218,7 +240,7 @@ Section GMPLemmas.
                 intros contra. apply Henv in contra. apply contra. simpl. StringSet.D.fsetdec.
             }
             apply not_in_sub_domain_prop in H1;[|apply in_domain_dec| apply in_domain_dec]. destruct H1.
-            * now unshelve epose proof (strong_reverse_dom_same_env ev' ev x a sub subrev Hsub1 Hsub2 Hrel _ H1).
+            * now unshelve epose proof (strong_reverse_dom_same_env ev' ev x a sub subrev Hbij Hrel _ H1).
             * exfalso. apply H1. now exists a.
 
             + eapply weakening_of_c_expression_semantics_3... split. 
@@ -232,20 +254,21 @@ Section GMPLemmas.
                 intros contra. apply Henv in contra. apply contra. simpl. StringSet.D.fsetdec.
                 }
                 apply not_in_sub_domain_prop in H2;[|apply in_domain_dec| apply in_domain_dec]. destruct H2.
-                * now unshelve epose proof (strong_reverse_dom_same_env ev' ev x a sub subrev Hsub1 Hsub2 Hrel _ H2).
+                * now unshelve epose proof (strong_reverse_dom_same_env ev' ev x a sub subrev Hbij Hrel _ H2).
                 * exfalso. apply H2. now exists a.
             + assert (~(dom ev - dom ev')%dom_ y). {
                 intros contra. apply Henv in contra. apply contra. simpl. StringSet.D.fsetdec.
                 }
                 apply not_in_sub_domain_prop in H2;[|apply in_domain_dec| apply in_domain_dec]. destruct H2.
-                * now unshelve epose proof (strong_reverse_dom_same_env ev' ev y n sub subrev Hsub1 Hsub2 Hrel _ H2).
+                * now unshelve epose proof (strong_reverse_dom_same_env ev' ev y n sub subrev Hbij Hrel _ H2).
                 * exfalso. apply H2. now exists n.
             + assert (~(dom ev.(mstate) - dom ev'.(mstate))%dom_ (subrev n)). {
-                intros contra. apply Hmem in contra. destruct contra. simpl in H2. destruct H2 as [H2 []].
-                rewrite Hsub2 in H2. assert (x0 = y). { admit. (* no aliasing *) } subst. StringSet.D.fsetdec.
-                } 
+                    intros contra. apply Hmem in contra. destruct contra. simpl in H2. destruct H2 as [H2 []].
+                    destruct Hbij as [? Hsub2]; rewrite Hsub2 in H2. assert (x0 = y). { admit. (* no aliasing *) } 
+                    subst. StringSet.D.fsetdec. 
+                }
                 apply not_in_sub_domain_prop in H2;[|apply in_domain_dec| apply in_domain_dec]. destruct H2.
-                * now unshelve epose proof (strong_reverse_dom_same_mem ev' ev _ z sub subrev Hsub1 Hsub2 Hrel _ H2).
+                * now unshelve epose proof (strong_reverse_dom_same_mem ev' ev _ z sub subrev Hbij Hrel _ H2).
                 * destruct H2. admit.
 
         - exists (ev' <| env ; vars ::= {{x\VInt (zy ⁱⁿᵗ ir) : 𝕍}} |>). apply S_get_int with (subrev ly).
@@ -253,15 +276,15 @@ Section GMPLemmas.
                 intros contra. apply Henv in contra. apply contra. simpl. StringSet.D.fsetdec.
                 }
                 apply not_in_sub_domain_prop in H1;[|apply in_domain_dec| apply in_domain_dec]. destruct H1.
-                * now  unshelve epose proof (strong_reverse_dom_same_env ev' ev y ly sub subrev Hsub1 Hsub2 Hrel _ H1).
+                * now  unshelve epose proof (strong_reverse_dom_same_env ev' ev y ly sub subrev Hbij Hrel _ H1).
                 * destruct H1. now exists ly.
 
             + assert (~(dom ev.(mstate) - dom ev'.(mstate))%dom_ (subrev ly)). {
                 intros contra. apply Hmem in contra. destruct contra. simpl in H1. destruct H1 as [H1 []].
-                rewrite Hsub2 in H1. assert (x0 = y). { admit. (* no aliasing *) } subst. StringSet.D.fsetdec.
+                    destruct Hbij as [? Hsub2]; rewrite Hsub2 in H1. assert (x0 = y). { admit. (* no aliasing *) } subst. StringSet.D.fsetdec.
                 } 
                 apply not_in_sub_domain_prop in H1;[|apply in_domain_dec| apply in_domain_dec]. destruct H1.
-                * now unshelve epose proof (strong_reverse_dom_same_mem ev' ev _ zy sub subrev Hsub1 Hsub2 Hrel _ H1).
+                * now unshelve epose proof (strong_reverse_dom_same_mem ev' ev _ zy sub subrev Hbij Hrel _ H1).
                 *  destruct H1. admit.
         
         - exists (ev' <| mstate ::= {{subrev lx\Defined zx}} |>). apply S_set_s...
@@ -269,7 +292,7 @@ Section GMPLemmas.
                 intros contra. apply Henv in contra. apply contra. simpl. StringSet.D.fsetdec.
                 }
                 apply not_in_sub_domain_prop in H1;[|apply in_domain_dec| apply in_domain_dec]. destruct H1.
-                * now  unshelve epose proof (strong_reverse_dom_same_env ev' ev x lx sub subrev Hsub1 Hsub2 Hrel _ H1).
+                * now  unshelve epose proof (strong_reverse_dom_same_env ev' ev x lx sub subrev Hbij Hrel _ H1).
                 * destruct H1. now exists lx.
 
 
@@ -278,28 +301,30 @@ Section GMPLemmas.
                 intros contra. apply Henv in contra. apply contra. simpl. StringSet.D.fsetdec.
                 }
                 apply not_in_sub_domain_prop in H4;[|apply in_domain_dec| apply in_domain_dec]. destruct H4.
-                * now  unshelve epose proof (strong_reverse_dom_same_env ev' ev x lx sub subrev Hsub1 Hsub2 Hrel _ H4).
+                * now  unshelve epose proof (strong_reverse_dom_same_env ev' ev x lx sub subrev Hbij Hrel _ H4).
                 * destruct H4. now exists lx.
             + assert (~(dom ev - dom ev')%dom_ y). {
                 intros contra. apply Henv in contra. apply contra. simpl. StringSet.D.fsetdec.
                 }
                 apply not_in_sub_domain_prop in H4;[|apply in_domain_dec| apply in_domain_dec]. destruct H4.
-                * now  unshelve epose proof (strong_reverse_dom_same_env ev' ev y ly sub subrev Hsub1 Hsub2 Hrel _ H4).
+                * now  unshelve epose proof (strong_reverse_dom_same_env ev' ev y ly sub subrev Hbij Hrel _ H4).
                 * destruct H4. now exists ly.
             + assert (~(dom ev.(mstate) - dom ev'.(mstate))%dom_ (subrev lx)). {
                 intros contra. apply Hmem in contra. destruct contra. simpl in H4. destruct H4 as [H4 []].
-                rewrite Hsub2 in H4. assert (x0 = y). { admit. (* no aliasing *) } subst. StringSet.D.fsetdec.
+                    destruct Hbij as [? Hsub2]; rewrite Hsub2 in H4. assert (x0 = y). { admit. (* no aliasing *) } subst. StringSet.D.fsetdec.
                 } 
                 apply not_in_sub_domain_prop in H4;[|apply in_domain_dec| apply in_domain_dec]. destruct H4.
-                * now unshelve epose proof (strong_reverse_dom_same_mem ev' ev _ zx sub subrev Hsub1 Hsub2 Hrel _ H4).
+                * now unshelve epose proof (strong_reverse_dom_same_mem ev' ev _ zx sub subrev Hbij Hrel _ H4).
                 *  destruct H4. admit.
             + assert (~(dom ev.(mstate) - dom ev'.(mstate))%dom_ (subrev ly)). {
                 intros contra. apply Hmem in contra. destruct contra. simpl in H4. destruct H4 as [H4 []].
-                rewrite Hsub2 in H4. assert (x0 = y). { admit. (* no aliasing *) } subst. StringSet.D.fsetdec.
+                     destruct Hbij as [? Hsub2]; rewrite Hsub2 in H4. assert (x0 = y). { admit. (* no aliasing *) } subst. StringSet.D.fsetdec.
                 } 
                 apply not_in_sub_domain_prop in H4;[|apply in_domain_dec| apply in_domain_dec]. destruct H4.
-                * now unshelve epose proof (strong_reverse_dom_same_mem ev' ev _ zy sub subrev Hsub1 Hsub2 Hrel _ H4).
-                *  destruct H4. admit.
+                * now unshelve epose proof (strong_reverse_dom_same_mem ev' ev _ zy sub subrev Hbij Hrel _ H4).
+                * destruct Hrel as [_ Hmem'].  specialize (Hmem' (subrev ly) zy). simpl in Hmem'. destruct Hbij as [? subsubrev]. 
+                    rewrite subsubrev in Hmem'. admit.
+                    
 
 
         - exists (ev'<| mstate ::= {{subrev lr\Defined (⋄ (□ bop) zx zy) }} |>). apply S_op with (subrev lx) (subrev ly).
@@ -307,7 +332,7 @@ Section GMPLemmas.
                 intros contra. apply Henv in contra. apply contra. simpl. destruct bop; simpl ; StringSet.D.fsetdec.
                 }
                 apply not_in_sub_domain_prop in H4;[|apply in_domain_dec| apply in_domain_dec]. destruct H4.
-                * now  unshelve epose proof (strong_reverse_dom_same_env ev' ev x lx sub subrev Hsub1 Hsub2 Hrel _ H4).
+                * now  unshelve epose proof (strong_reverse_dom_same_env ev' ev x lx sub subrev Hbij Hrel _ H4).
                 * destruct H4. now exists lx.
 
             
@@ -315,36 +340,36 @@ Section GMPLemmas.
                 intros contra. apply Henv in contra. apply contra. simpl. destruct bop; simpl ; StringSet.D.fsetdec.
                 }
                 apply not_in_sub_domain_prop in H4;[|apply in_domain_dec| apply in_domain_dec]. destruct H4.
-                * now  unshelve epose proof (strong_reverse_dom_same_env ev' ev y ly sub subrev Hsub1 Hsub2 Hrel _ H4).
+                * now  unshelve epose proof (strong_reverse_dom_same_env ev' ev y ly sub subrev Hbij Hrel _ H4).
                 * destruct H4. now exists ly.
 
             + assert (~(dom ev.(mstate) - dom ev'.(mstate))%dom_ (subrev lx)). {
                 intros contra. apply Hmem in contra. destruct contra. simpl in H4. destruct H4 as [H4 []].
-                rewrite Hsub2 in H4. assert (x0 = y). { admit. (* no aliasing *) } subst. destruct bop; simpl ; StringSet.D.fsetdec.
+                     destruct Hbij as [? Hsub2]; rewrite Hsub2 in H4. assert (x0 = y). { admit. (* no aliasing *) } subst. destruct bop; simpl ; StringSet.D.fsetdec.
                 } 
                 apply not_in_sub_domain_prop in H4;[|apply in_domain_dec| apply in_domain_dec]. destruct H4.
-                * now unshelve epose proof (strong_reverse_dom_same_mem ev' ev _ zx sub subrev Hsub1 Hsub2 Hrel _ H4).
-                *  destruct H4. admit.
+                * now unshelve epose proof (strong_reverse_dom_same_mem ev' ev _ zx sub subrev Hbij Hrel _ H4).
+                *  destruct H4.  admit.
 
             + assert (~(dom ev.(mstate) - dom ev'.(mstate))%dom_ (subrev ly)). {
                 intros contra. apply Hmem in contra. destruct contra. simpl in H4. destruct H4 as [H4 []].
-                rewrite Hsub2 in H4. assert (x0 = y). { admit. (* no aliasing *) } subst. destruct bop; simpl ; StringSet.D.fsetdec.
+                     destruct Hbij as [? Hsub2]; rewrite Hsub2 in H4. assert (x0 = y). { admit. (* no aliasing *) } subst. destruct bop; simpl ; StringSet.D.fsetdec.
                 } 
                 apply not_in_sub_domain_prop in H4;[|apply in_domain_dec| apply in_domain_dec]. destruct H4.
-                * now unshelve epose proof (strong_reverse_dom_same_mem ev' ev _ zy sub subrev Hsub1 Hsub2 Hrel _ H4).
+                * now unshelve epose proof (strong_reverse_dom_same_mem ev' ev _ zy sub subrev Hbij Hrel _ H4).
                 *  destruct H4. admit.
             
             + assert (~(dom ev - dom ev')%dom_ r). {
                 intros contra. apply Henv in contra. apply contra. simpl. destruct bop; simpl ; StringSet.D.fsetdec.
                 }
                 apply not_in_sub_domain_prop in H4;[|apply in_domain_dec| apply in_domain_dec]. destruct H4.
-                * now  unshelve epose proof (strong_reverse_dom_same_env ev' ev _ lr sub subrev Hsub1 Hsub2 Hrel _ H4).
+                * now  unshelve epose proof (strong_reverse_dom_same_env ev' ev _ lr sub subrev Hbij Hrel _ H4).
                 * destruct H4. now exists lr.                
     Admitted.
 
 
     Definition LC23_weakening_of_gmp_statement_semantics := 
-        LC23_weakening_of_statement_semantics Empty_exp_sem  _gmp_stmt_sem 
+        LC23_weakening_of_statement_semantics_strong Empty_exp_sem  _gmp_stmt_sem 
         (weakening_of_empty_expression_semantics_3 strong_env_mem_partial_order) 
         _LC23_weakening_of_gmp_statement_semantics
         (ext_used_stmt_vars:=_gmp_used_stmt_vars) (ext_ty_val:=_type_of_gmp)
